Removed all cheats from ffi_irrel proof tree except ffi_gets_stream - all hinges on this now!

projection/proofs/to_cake/ffi/comms_ffi_rec_characScript.sml
@@ -527,6 +527,335 @@ Proof
       metis_tac[ffi_eq_def,BISIM_REL_def,BISIM_def])
 QED
 
+Definition netout_trans_def:
+  netout_trans conf c n1 n2 ⇔
+    ∃sp d. trans conf n1 (LSend sp d c) n2
+End
+
+Definition netin_trans_def:
+  netin_trans conf c n1 n2 ⇔
+    (∃L. trans conf n1 L n2 ∧
+      ∀sp d. L ≠ LSend sp d c)
+End
+
+Definition netout_limit_def:
+  (netout_limit conf c n1 0 ⇔
+    ¬∃n2 n3.
+      RTC (netin_trans conf c) n1 n2 ∧
+      netout_trans conf c n2 n3) ∧
+  (netout_limit conf c n1 (SUC i) ⇔
+    (∃n2 n3.
+      RTC (netin_trans conf c) n1 n2 ∧
+      netout_trans conf c n2 n3) ∧
+    (∀n2 n3.
+      RTC (netin_trans conf c) n1 n2 ∧
+      netout_trans conf c n2 n3 ⇒
+      netout_limit conf c n3 i)) 
+End
+
+Theorem netin_struc_pres_NNil:
+  ∀conf c n2.
+    RTC (netin_trans conf c) NNil n2 ⇒
+    n2 = NNil
+Proof
+  rw[] >> pop_assum mp_tac >>
+  qid_spec_tac ‘n2’ >>
+  Induct_on ‘RTC’ >> rw[] >>
+  fs[netin_trans_def] >> fs[Once trans_cases]
+QED
+
+Theorem netin_struc_pres_NPar:
+  ∀conf n1a n1b n2.
+    RTC (netin_trans conf c) (NPar n1a n1b) n2 ⇒
+    ∃n2a n2b.
+      n2 = NPar n2a n2b
+Proof
+  rw[] >> pop_assum mp_tac >>
+  MAP_EVERY qid_spec_tac [‘n1a’,‘n1b’,‘n2’] >>
+  Induct_on ‘RTC’ >> rw[] >>
+  fs[netin_trans_def] >> fs[Once trans_cases]
+QED
+
+Theorem netin_struc_prop_NPar:
+  ∀conf c n1a n1b n2a n2b.
+    ¬(net_has_node (NPar n1a n1b) c) ∧
+    RTC (netin_trans conf c) (NPar n1a n1b) (NPar n2a n2b) ⇒
+    (RTC (netin_trans conf c) n1a n2a ∧
+     RTC (netin_trans conf c) n1b n2b)
+Proof
+  ntac 2 strip_tac >> Induct_on ‘RTC’ >> rw[]
+  >- rw[RTC_REFL] >- rw[RTC_REFL] >>
+  rename1 ‘netin_trans conf c (NPar n1a n1b) ni’ >>
+  ‘∃nia nib. ni = NPar nia nib’
+    by metis_tac[RTC_SINGLE,netin_struc_pres_NPar] >>
+  ‘¬net_has_node ni c’
+    by (fs[netin_trans_def] >> metis_tac[trans_pres_nodes])  >>
+  rw[]
+  >- (‘RC (netin_trans conf c) n1a nia’
+        suffices_by (rw[RC_DEF] >>
+                     metis_tac[RTC_REFL,RTC_SINGLE,RTC_TRANSITIVE,
+                           transitive_def]) >>
+      fs[netin_trans_def,netout_trans_def] >>
+      last_x_assum (assume_tac o REWRITE_RULE [Once trans_cases]) >>
+      fs[] >> rw[RC_DEF] >> fs[netin_trans_def]
+      >- (DISJ2_TAC >>
+          rename1 ‘trans conf _ (LSend p1 d p2) _’ >>
+          qexists_tac ‘LSend p1 d p2’ >> rw[] >>
+          DISJ2_TAC >> DISJ2_TAC >>
+          ‘net_has_node n1b p2’
+            suffices_by (fs[net_has_node_def] >> metis_tac[]) >>
+          metis_tac[trans_receive_cond])
+      >- (DISJ2_TAC >>
+          rename1 ‘trans conf _ (LReceive p1 d p2) _’ >>
+          qexists_tac ‘LReceive p1 d p2’ >> fs[])
+      >- metis_tac[])
+  >- (‘RC (netin_trans conf c) n1b nib’
+        suffices_by (rw[RC_DEF] >>
+                     metis_tac[RTC_REFL,RTC_SINGLE,RTC_TRANSITIVE,
+                           transitive_def]) >>
+      fs[netin_trans_def,netout_trans_def] >>
+      last_x_assum (assume_tac o REWRITE_RULE [Once trans_cases]) >>
+      fs[] >> rw[RC_DEF] >> fs[netin_trans_def]
+      >- (DISJ2_TAC >>
+          rename1 ‘trans conf _ (LReceive p1 d p2) _’ >>
+          qexists_tac ‘LReceive p1 d p2’ >> fs[])
+      >- (DISJ2_TAC >>
+          rename1 ‘trans conf _ (LSend p1 d p2) _’ >>
+          qexists_tac ‘LSend p1 d p2’ >> rw[] >>
+          DISJ2_TAC >> DISJ2_TAC >>
+          ‘net_has_node n1a p2’
+            suffices_by (fs[net_has_node_def] >> metis_tac[]) >>
+          metis_tac[trans_receive_cond])
+      >- metis_tac[])
+QED
+
+Theorem netin_struc_pres_NEndpoint:
+  ∀conf c p s e n2.
+    RTC (netin_trans conf c) (NEndpoint p s e) n2 ⇒
+    ∃s2 e2.
+      n2 = NEndpoint p s2 e2
+Proof
+  rw[] >> pop_assum mp_tac >>
+  MAP_EVERY qid_spec_tac [‘s’,‘e’,‘n2’] >>
+  Induct_on ‘RTC’ >> rw[] >>
+  fs[netin_trans_def] >> fs[Once trans_cases]
+QED
+
+Theorem netout_limit_exists:
+  ∀conf c net.
+    ¬net_has_node net c ⇒
+    ∃n.
+      netout_limit conf c net n
+Proof
+  ntac 2 strip_tac >> Induct_on ‘net’ >> rw[]
+  >- (qexists_tac ‘0’ >> rw[netout_limit_def] >>
+      reverse (Cases_on ‘RTC (netin_trans conf c) NNil n2’) >>
+      rw[] >>
+      ‘n2 = NNil’
+        suffices_by rw[netout_trans_def, Once trans_cases] >> 
+      metis_tac[netin_struc_pres_NNil])
+  >- (fs[net_has_node_def] >>
+      rename[‘NPar net1 net2’,‘netout_limit conf c net1 i1’,
+             ‘netout_limit conf c net2 i2’] >>
+      qexists_tac ‘i1 + i2’ >> rpt (pop_assum mp_tac) >>
+      MAP_EVERY qid_spec_tac [‘i2’,‘i1’,‘net2’,‘net1’] >>
+      Induct_on ‘i1’ >> Induct_on ‘i2’ >> rw[netout_limit_def]
+      >- (CCONTR_TAC >> fs[] >>
+          drule_all_then strip_assume_tac netin_struc_pres_NPar >>
+          fs[] >>
+          drule_all_then strip_assume_tac
+                        (REWRITE_RULE [net_has_node_def,boolTheory.DE_MORGAN_THM]
+                                      netin_struc_prop_NPar) >>
+          ‘(∃n3a. netout_trans conf c n2a n3a) ∨
+           (∃n3b. netout_trans conf c n2b n3b)’
+            suffices_by (rw[] >> metis_tac[]) >>
+          qpat_x_assum ‘netout_trans _ _ _ _’ (assume_tac o REWRITE_RULE [netout_trans_def]) >>
+          rw[] >> fs[Once trans_cases] >> rw[netout_trans_def] >> metis_tac[])
+      >- (qexistsl_tac [‘NPar net1 n2’,‘NPar net1 n3’] >>
+          reverse (rw[netout_trans_def])
+          >- (rw[Once trans_cases] >> fs[netout_trans_def] >> metis_tac[]) >>
+          qpat_x_assum ‘RTC _ _ _’ mp_tac >>
+          MAP_EVERY qid_spec_tac [‘net2’,‘n2’] >>
+          Induct_on ‘RTC’ >> rw[] >>
+          rename1 ‘netin_trans conf c net2ia net2ib’ >>
+          ‘netin_trans conf c (NPar net1 net2ia) (NPar net1 net2ib)’
+            suffices_by metis_tac[RTC_SINGLE,RTC_TRANSITIVE,transitive_def] >>
+          rw[netin_trans_def,Once trans_cases] >> fs[netin_trans_def] >>
+          metis_tac[])
+      >- (drule_all_then strip_assume_tac netin_struc_pres_NPar >>
+          fs[] >> rename1 ‘netout_trans conf c (NPar n2a n2b) n3P’ >>
+          ‘∃n3a n3b. n3P = NPar n3a n3b’
+            by (fs[netout_trans_def] >> fs[Once trans_cases] >> rw[]) >>
+          fs[] >> last_x_assum irule >> rw[]
+          >- (‘¬net_has_node (NPar n3a n3b) c’
+                suffices_by rw[net_has_node_def] >>
+              ‘¬net_has_node (NPar n2a n2b) c’
+                suffices_by  (fs[netout_trans_def] >> metis_tac[trans_pres_nodes]) >>
+              ‘¬net_has_node (NPar net1 net2) c’
+                suffices_by (qpat_x_assum ‘RTC _ _ _’ mp_tac >>
+                             MAP_EVERY qid_spec_tac [‘net1’,‘net2’,‘n2a’,‘n2b’] >>
+                             Induct_on ‘RTC’ >> rw[] >>
+                             pop_assum irule >>
+                             fs[netin_trans_def,Once trans_cases,net_has_node_def] >>
+                             metis_tac[trans_pres_nodes]) >>
+              rw[net_has_node_def])
+          >- (‘¬net_has_node (NPar n3a n3b) c’
+                suffices_by rw[net_has_node_def] >>
+              ‘¬net_has_node (NPar n2a n2b) c’
+                suffices_by  (fs[netout_trans_def] >> metis_tac[trans_pres_nodes]) >>
+              ‘¬net_has_node (NPar net1 net2) c’
+                suffices_by (qpat_x_assum ‘RTC _ _ _’ mp_tac >>
+                             MAP_EVERY qid_spec_tac [‘net1’,‘net2’,‘n2a’,‘n2b’] >>
+                             Induct_on ‘RTC’ >> rw[] >>
+                             pop_assum irule >>
+                             fs[netin_trans_def,Once trans_cases,net_has_node_def] >>
+                             metis_tac[trans_pres_nodes]) >>
+              rw[net_has_node_def])
+          >- (fs[netout_trans_def] >>
+              qpat_x_assum ‘trans _ (NPar _ _) _ (NPar _ _)’
+                           (assume_tac o REWRITE_RULE [Once trans_cases]) >>
+              fs[]
+              >- (last_x_assum (qspec_then ‘n2a’ strip_assume_tac) >>
+                  ‘RTC (netin_trans conf c) net1 n2a’
+                    by (drule_all_then strip_assume_tac
+                                       (REWRITE_RULE [net_has_node_def,boolTheory.DE_MORGAN_THM]
+                                                      netin_struc_prop_NPar)) >>
+                  metis_tac[]) >>
+              rw[netout_limit_def] >> rename1 ‘¬RTC (netin_trans conf c) n2a NI’ >>
+              Cases_on ‘RTC (netin_trans conf c) n2a NI’ >> rw[] >>
+              last_x_assum (qspec_then ‘NI’ strip_assume_tac) >>
+              ‘RTC (netin_trans conf c) net1 NI’
+                by (drule_all_then strip_assume_tac
+                                   (REWRITE_RULE [net_has_node_def,boolTheory.DE_MORGAN_THM]
+                                                  netin_struc_prop_NPar) >>
+                    metis_tac[RTC_TRANSITIVE,transitive_def]) >>
+              fs[] >> rw[netout_trans_def])
+          >- (fs[netout_trans_def] >>
+              qpat_x_assum ‘trans _ (NPar _ _) _ (NPar _ _)’
+                           (assume_tac o REWRITE_RULE [Once trans_cases]) >>
+              reverse (fs[])
+              >- (last_x_assum (qspec_then ‘n2b’ strip_assume_tac) >>
+                  ‘RTC (netin_trans conf c) net2 n2b’
+                    by (drule_all_then strip_assume_tac
+                                       (REWRITE_RULE [net_has_node_def,boolTheory.DE_MORGAN_THM]
+                                                      netin_struc_prop_NPar)) >>
+                  metis_tac[]) >>
+              last_x_assum (qspec_then ‘n2a’ strip_assume_tac) >>
+              ‘RTC (netin_trans conf c) net1 n2a’
+                by (drule_all_then strip_assume_tac
+                                   (REWRITE_RULE [net_has_node_def,boolTheory.DE_MORGAN_THM]
+                                                  netin_struc_prop_NPar) >>
+                    metis_tac[RTC_TRANSITIVE,transitive_def]) >>
+              fs[] >> rw[netout_trans_def])
+            )
+          >- cheat
+          >- cheat
+          >- cheat
+          )
+      >- cheat
+QED
+
+Theorem netout_limit_unique:
+  ∀conf c N n m.
+    netout_limit conf c N m ∧
+    netout_limit conf c N n ⇒
+    (m = n)
+Proof
+  ntac 2 strip_tac >>
+  Induct_on ‘m’ >> Induct_on ‘n’ >>
+  rw[netout_limit_def]
+  >- metis_tac[]
+  >- metis_tac[] >>
+  first_x_assum irule >>
+  ntac 2 (first_x_assum (drule_all_then assume_tac)) >>
+  metis_tac[]
+QED
+
+Theorem netout_limit_cond:
+  ∀conf c n1 i.
+    ¬net_has_node n1 c ∧
+    (∃n2 n3.
+      RTC (netin_trans conf c) n1 n2 ∧
+      netout_trans conf c n2 n3 ∧
+      netout_limit conf c n3 i) ⇒
+    (netout_limit conf c n1 (SUC i)) 
+Proof
+  rpt strip_tac >> CCONTR_TAC >>
+  ‘∃m. netout_limit conf c n1 m’
+    by metis_tac[netout_limit_exists] >>
+  Cases_on ‘m = SUC i’ >> fs[] >> Cases_on ‘m’ >>
+  fs[netout_limit_def]
+  >- metis_tac[] >>
+  pop_assum mp_tac >> simp[] >>
+  rename1 ‘netout_limit conf c NF i’ >>
+  ‘netout_limit conf c NF n’
+    suffices_by metis_tac[netout_limit_unique] >>
+  first_x_assum irule >> metis_tac[]
+QED
+
+(*
+Theorem active_trans_netout_limit_same:
+  ∀conf c qA NA qB NB.
+    RTC (active_trans conf c) (qA,NA) (qB,NB) ⇒
+    ¬net_has_node NA c ⇒
+    qsame qA qB ⇒
+    netout_limit conf c NA = netout_limit conf c NB
+Proof
+  ntac 2 strip_tac >>
+  Induct_on ‘RTC’ >> rw[] >>
+  rename1 ‘active_trans conf c (qA,NA) NI’ >>
+  PairCases_on ‘NI’ >> rename1 ‘active_trans conf c (qA,NA) (qI,NI)’ >>
+  first_x_assum (qspecl_then [‘qI’,‘NI’] assume_tac) >>
+  fs[] >>
+  ‘¬net_has_node NI c’
+    by (fs[active_trans_def,internal_trans_def,emit_trans_def] >>
+        metis_tac[trans_pres_nodes]) >>
+  ‘qsame qI qB’
+    by (rw[qsame_def] >>
+        rename1 ‘qlk _ sp = qlk _ sp’ >> 
+        ‘isPREFIX (qlk qI sp) (qlk qB sp) ∧ isPREFIX (qlk qB sp) (qlk qI sp)’
+          suffices_by metis_tac[IS_PREFIX_ANTISYM] >>
+        rw[]
+        >- metis_tac[active_trans_queue_expand] >>
+        ‘isPREFIX (qlk qA sp) (qlk qI sp)’
+          suffices_by fs[qsame_def] >>
+        metis_tac[RTC_SINGLE,active_trans_queue_expand]) >>
+  fs[] >>
+  ‘netout_limit conf c NA = netout_limit conf c NI’
+    suffices_by metis_tac[] >>
+  qpat_x_assum ‘netout_limit conf c NI = _’ kall_tac >>
+  ‘internal_trans conf c (qA,NA) (qI,NI)’
+    by (fs[active_trans_def,emit_trans_def] >> CCONTR_TAC >> fs[] >>
+        ‘qsame qA qI’
+          suffices_by (rw[qsame_def] >> rename1 ‘qpush qA sp d’ >>
+                       qexists_tac ‘sp’ >> rw[]) >>
+        fs[qsame_def] >> metis_tac[]) >>
+  rpt (qpat_x_assum ‘qsame _ _’ kall_tac) >>
+  rpt (qpat_x_assum ‘active_trans _ _ _ _’ kall_tac) >>
+  rpt (qpat_x_assum ‘RTC (active_trans _ _) _ _’ kall_tac) >>
+  fs[internal_trans_def] >>
+  rw[FUN_EQ_THM,EQ_IMP_THM,netout_limit_def]
+  >- (CCONTR_TAC >>
+      rename1 ‘netout_limit conf c NA x’ >>
+      Cases_on ‘x’
+      >- (fs[netout_limit_def] >> CCONTR_TAC >>
+          fs[] >> qpat_x_assum ‘∀n2 n3. ¬RTC _ _ n2 ∨ ¬_ _ _ n2 n3’ mp_tac >>
+          simp[] >> rename [‘RTC (netin_trans conf c) NI N2’,‘netout_trans conf c N2 N3’] >>
+          qexistsl_tac [‘N2’,‘N3’] >>
+          ‘netin_trans conf c NA NI’
+            suffices_by (rw[] >> metis_tac[RTC_SINGLE,RTC_TRANSITIVE,transitive_def]) >>
+          rw[netin_trans_def] >> qexists_tac ‘LTau’ >> rw[]) >>
+      ‘∃y. netout_limit conf c NI y’
+        by metis_tac[netout_limit_exists] >>
+      rename1 ‘SUC n’ >>
+      Cases_on ‘y = SUC n’ >> fs[] >>
+      ‘netout_limit conf c NA y’
+        suffices_by (rw[] >> metis_tac[met]
+      
+
+
+  first_x_assum (drul)
+QED*)
 
 Theorem ffi_gets_stream:
   ∀conf src (st : total_state ffi_state).
@@ -536,8 +865,111 @@ Theorem ffi_gets_stream:
      (∃cs. ffi_divg_stream conf st src cs) ∨
      (∃cs. ffi_fail_stream conf st src cs))
 Proof
+  cheat
+(*
   rw[] >>
-  reverse (Induct_on ‘qlk ((λ(_,q,_).q) st.ffi_state) src’)
+  ‘∃c q N. st.ffi_state = (c,q,N)’
+    by (rename1 ‘ffi_wf ffiSt’ >> PairCases_on ‘ffiSt’ >> rw[]) >>
+  fs[] >>
+  ‘∃n. netout_limit conf c N n’
+    by (irule netout_limit_exists >>
+        fs[ffi_wf_def]) >>
+  rpt (pop_assum mp_tac) >>
+  MAP_EVERY qid_spec_tac [‘st’,‘N’] >>
+  Induct_on ‘n’ >>
+  Induct_on ‘qlk q src’
+  (* Handle empty queue and netout_limit 0 *)
+  >- (rw[] >> DISJ2_TAC >> DISJ1_TAC >>
+      qexists_tac ‘[]’ >>
+      rw[ffi_divg_stream_def,call_FFI_def,
+         comms_ffi_oracle_def,valid_receive_call_format_def,
+         ffi_receive_def,some_def,AllCaseEqs()] >>
+      rename1 ‘¬_ x’ >> PairCases_on ‘x’ >>
+      rw[] >> CCONTR_TAC >> fs[] >>
+      ‘x1 = c’
+        by metis_tac[strans_pres_pnum,pairTheory.FST] >>
+      rw[] >>
+      drule_all_then strip_assume_tac strans_receive_deconstruct >>
+      ‘qi1 ≠ q’
+        by (CCONTR_TAC >> fs[output_trans_def] >>
+            ‘qlk (normalise_queues q) src = qlk (normalise_queues qi2 |+ (src,x0::qlk qi2 src)) src’
+              by (qpat_x_assum ‘normalise_queues q = _’ SUBST1_TAC >> rw[]) >>
+            fs[]) >>
+      ‘∃n. netout_limit conf c N (SUC n)’
+        suffices_by (strip_tac >> fs[] >>
+                     ‘SUC n = 0’
+                        suffices_by rw[] >>
+                     metis_tac[netout_limit_unique]) >>
+      pop_assum mp_tac >>
+      rename1 ‘RTC (active_trans conf c) (q,N) (qi1,ni)’ >>
+      qpat_x_assum ‘ffi_wf (c,q,N)’ mp_tac >>
+      qpat_x_assum ‘RTC (active_trans conf c) (q,N) (qi1,ni)’ mp_tac >>
+      MAP_EVERY qid_spec_tac [‘q’,‘N’,‘qi1’,‘ni’] >>
+      Induct_on ‘RTC’ >> rw[] >> rename1 ‘active_trans conf c (qA,NA) qNB’ >>
+      PairCases_on ‘qNB’ >> rename1 ‘RTC (active_trans conf c) (qB,NB) (qC,NC)’ >>
+      ‘ffi_wf (c,qB,NB)’
+        by metis_tac[RTC_SINGLE,active_trans_pres_wf] >>
+      fs[active_trans_def,internal_trans_def,emit_trans_def]
+      >- (qpat_x_assum ‘_ ⇒ ∃n. _’ mp_tac >> impl_tac >- metis_tac[] >> rw[] >>
+          rename1 ‘netout_limit conf c NB (SUC n)’ >>
+          qexists_tac ‘n’ >>
+          irule netout_limit_cond >>
+          reverse (rw[])
+          >- fs[ffi_wf_def] >>
+          pop_assum (assume_tac o REWRITE_RULE [netout_limit_def]) >>
+          fs[]
+          rename [‘RTC (netin_trans conf c) NB NI’,‘netout_trans conf c NI NE’] >>
+          qexistsl_tac [‘NI’,‘NE’] >> reverse (rw[])
+          >- metis_tac[] >>
+          ‘netin_trans conf c NA NB’
+            suffices_by metis_tac[RTC_SINGLE,RTC_TRANSITIVE,transitive_def] >>
+          rw[netin_trans_def] >> qexists_tac ‘LTau’ >> rw[])
+
+          ‘∃m. netout_limit conf c NA m’
+            by (irule netout_limit_exists >>
+                fs[ffi_wf_def]) >>
+          Cases_on ‘m = n’ >> fs[] >> Cases_on ‘n’ >> Cases_on ‘m’ >>
+          fs[netout_limit_def] 
+          >- (rename [‘RTC (netin_trans conf c) NB NI’,‘netout_trans conf c NI NE’] >>
+              first_x_assum (qspecl_then [‘NI’,‘NE’] assume_tac) >>
+              rfs[] >>
+              ‘netin_trans conf c NA NB’
+                suffices_by metis_tac[RTC_SINGLE,RTC_TRANSITIVE,transitive_def] >>
+              rw[netin_trans_def] >> qexists_tac ‘LTau’ >> rw[]) >>
+          rpt (qpat_x_assum ‘RTC _ NA _’ kall_tac) >>
+          rename [‘RTC (netin_trans conf c) NB NI’,‘netout_trans conf c NI NE’] >>
+          first_x_assum (qspecl_then [‘NI’,‘NE’] mp_tac) >>
+          impl_tac
+          >- (rw[] >>
+              ‘netin_trans conf c NA NB’
+                suffices_by metis_tac[RTC_SINGLE,RTC_TRANSITIVE,transitive_def] >>
+              rw[netin_trans_def] >> qexists_tac ‘LTau’ >> rw[]) >>
+          rw[] >> first_x_assum (drule_all_then assume_tac) >>
+          CCONTR_TAC >> fs[] >>
+          qpat_x_assum ‘_ ≠ _’ mp_tac >> simp[] >>
+          metis_tac[netout_limit_unique])
+
+              )
+          ‘m ≠ 0’
+            by (CCONTR_TAC >> Cases_on ‘n’ >> fs[netout_limit_def]
+           Cases_on ‘n’ >>
+
+          ‘∃n2 n3.
+            RTC (netin_trans conf c)’
+                ‘ffi_wf’
+
+           Cases_on ‘n’ >> rw[netout_limit_def] >>
+          fs[]
+          >- (fs[netout_limit_def] >>
+              rename [‘RTC (netin_trans conf c) NB NI’,‘netout_trans conf c NI NE’] >>
+              MAP_EVERY qexists_tac [‘NI’,‘NE’] >> rw[] >>
+              ‘netin_trans conf c NA NB’
+                suffices_by metis_tac[RTC_SINGLE,RTC_TRANSITIVE,transitive_def] >>
+              fs[netin_trans_def] >> qexists_tac ‘LTau’ >> rw[]) >>
+          CCONTR_TAC
+          ‘qC ≠ qB’
+            by metis_tac[] >>
+          )
   (* Handle non-empty queue inductively *)
   >- (rw[] >> qabbrev_tac ‘fs = st.ffi_state’ >>
       PairCases_on ‘fs’ >> rename1 ‘(c,q,N)’ >> rename1 ‘h::tl’ >>
@@ -661,7 +1093,18 @@ Proof
           >- (qexists_tac ‘(h,(c,normalise_queues (q|+(src,tl)),N))’ >>
               rw[] >> metis_tac[strans_rules]))) >>
   (* Handle base case empty queue by induction on network *)
-  rw[] >> Induct_on ‘(λ(x,y,z). z) st.ffi_state’
+  rw[] >>
+  qspecl_then [‘conf’,‘(λ(c,_,_). c) st.ffi_state’, ‘(λ(_,_,n). n) st.ffi_state’]
+              assume_tac netout_limit_exists >>
+  pop_assum mp_tac >> impl_tac
+  >- (rename1 ‘(λ(_,_,n).n) ffist’ >> PairCases_on ‘ffist’ >> fs[ffi_wf_def]) >>
+  qabbrev_tac ‘c = (λ(c,_,_).c) st.ffi_state’ >>
+  qabbrev_tac ‘q = (λ(_,q,_).q) st.ffi_state’ >>
+  qabbrev_tac ‘N = (λ(_,_,n).n) st.ffi_state’ >>
+  rw[] >> Induct_on ‘n’
+  >- (rw[] >> DISJ2_TAC >> DISJ1_TAC >> qexists_tac ‘[]’ >> rw[ffi_divg_stream_def] >>
+      
+  Induct_on ‘(λ(x,y,z). z) st.ffi_state’
   (* Empty queue, Empty Network *)
   >- (rw[] >> DISJ2_TAC >> DISJ1_TAC >> qexists_tac ‘[]’ >>
       rw[ffi_divg_stream_def,call_FFI_def,valid_receive_call_format_def,
@@ -789,6 +1232,7 @@ Proof
       (* IfThen case *)
       >- cheat
       >- cheat)
+*)
 QED
 
 val _ = export_theory ();
